some cleaning

type/global.v
@@ -138,25 +138,229 @@ Proof.
         apply IHm; try easy.
 Qed.
 
-CoFixpoint Ga : gtt := gtt_send "Alice" "Bob" [Some (snat, Ga)].
-
-Example Grec : gttTC (g_rec (g_send "Alice" "Bob" [Some (snat, g_var 0)])) Ga.
+ 
+Lemma subst_injG : forall m n G G1 Q Q0, subst_global m n G G1 Q0 -> subst_global m n G G1 Q -> Q = Q0.
 Proof.
-  pcofix CIH.
-  pfold. apply gttT_rec with (Q := g_send "Alice" "Bob" [(Some (snat, (g_rec (g_send "Alice" "Bob" [Some (snat, g_var 0)]))))]).
-  constructor. constructor. right.
-  exists snat. exists (g_var 0). exists (g_rec (g_send "Alice" "Bob" [Some (snat, g_var 0)])).
-  split; try easy. split; try easy. constructor. easy.
+  intros m n G G1. revert m n G.
+  induction G1 using global_ind_ref; intros; try easy.
+  inversion H. subst. 
+  - inversion H0; try easy. 
+  - subst. inversion H0; try easy.
+  - subst. inversion H0; try easy.
+    subst. specialize(triad_le m t' H6 H8); try easy.
+  - subst. inversion H0; try easy. 
+    subst. specialize(triad_le m t' H8 H6); try easy.
   
-  rewrite (gtt_eq Ga). simpl.
-  left. pfold.
-  constructor. constructor. right. exists snat. exists (g_rec (g_send "Alice" "Bob" [Some (snat, g_var 0)])). exists Ga.
-  split; try easy. split; try easy.
-  right. easy. easy.
+  inversion H. subst. inversion H0. subst. easy.
+  
+  inversion H0. subst. inversion H1. subst.
+  assert (ys0 = ys). {
+    clear H0 H1. revert H H9 H10. revert p m n G ys ys0.
+    induction lis; intros; try easy.
+    destruct ys; try easy. destruct ys0; try easy.
+    destruct ys; try easy. destruct ys0; try easy.
+    inversion H. subst. clear H.
+    inversion H9. subst. clear H9.
+    inversion H10. subst. clear H10.
+    specialize(IHlis p m n G ys ys0 H3 H6 H8). subst.
+    clear H3 H6 H8.
+    destruct H4. destruct H. subst.
+    destruct H5. destruct H. subst. easy.
+    destruct H. destruct H. destruct H. easy.
+    destruct H. destruct H. destruct H. destruct H. destruct H0. subst.
+    destruct H5; try easy.
+    destruct H. destruct H. destruct H. destruct H. destruct H0. 
+    inversion H. subst. 
+    destruct H2; try easy. destruct H0. destruct H0. destruct H0. 
+    inversion H0. subst.
+    specialize(H2 m n G x1 x4 H3 H1). subst. easy.
+  }
+  subst. easy.
+  
+  inversion H. subst. inversion H0. subst.
+  specialize(IHG1 (S m) (S n) G Q1 Q0 H6 H5). subst. easy.
+Qed.
+
+Lemma wfG_after_incr : forall G1 m n,
+     wfG G1 -> wfG (incr_freeG m n G1).
+Proof.
+  induction G1 using global_ind_ref; intros; try easy.
+  - simpl in *.
+    constructor.
+  - revert m n H0 H. revert p.
+    induction lis; intros; try easy.
+    - inversion H. subst. clear H.
+      inversion H0. subst. inversion H7. subst. clear H7.
+      specialize(SList_f a lis H5); intros.
+      destruct H.
+      - assert (wfG (incr_freeG m n (g_send p q lis))).
+        {
+          apply IHlis; try easy.
+          inversion H0. subst.
+          constructor; try easy.
+        }
+        destruct H2. subst.
+        - constructor. 
+          {
+            simpl. clear IHlis H3 H0 H4 H5 H6 H1. 
+            revert m n p H. induction lis; intros; try easy.
+            specialize(SList_f a lis H); intros.
+            destruct H0.
+            - apply SList_b. apply IHlis; try easy. inversion H8. easy.
+            - destruct H0. destruct H1. subst. 
+            simpl. destruct x; try easy.
+          }
+          easy.
+          {
+            clear IHlis H3 H0 H5 H1 H6. 
+            revert H H4 H8. revert m n. clear q p.
+            induction lis; intros; try easy. constructor. left. easy.
+            - specialize(SList_f a lis H); intros.
+              inversion H4. subst. clear H4. inversion H8. subst. clear H8.
+              destruct H0. specialize(IHlis m n H0 H5 H6). inversion IHlis. subst. clear IHlis.
+              constructor; try easy. clear H8. clear H7 H6 H5.
+              destruct H3. subst. left. easy.
+              destruct H1. destruct H1. destruct H1. subst. right.
+              exists x. exists (incr_freeG m n x0). split; try easy.
+              destruct H4; try easy. apply H2; try easy.
+              destruct H1. destruct H1. destruct H1. inversion H1. subst. easy.
+              
+            - destruct H0. destruct H1. subst. constructor; try easy.
+              right. destruct x. exists s. 
+              destruct H3; try easy. destruct H0. destruct H0. destruct H0. inversion H0. subst.
+              destruct H4; try easy. destruct H2. destruct H2. destruct H2. inversion H2. subst.
+              exists (incr_freeG m n x2). split; try easy. apply H1; try easy.
+          }
+        - destruct H2. destruct H2. destruct H2. subst. 
+          constructor; try easy.
+          {
+             apply SList_b.
+             clear IHlis H3 H0 H4 H5 H6 H7 H8 H1. clear x x0 p q.
+             revert m n H.
+             induction lis; intros; try easy.
+             specialize(SList_f a lis H); intros.
+             destruct H0. apply SList_b. apply IHlis; try easy.
+             destruct H0. destruct H1. subst. destruct x. easy.
+          }
+          constructor. right. exists x. exists (incr_freeG m n x0).
+          split; try easy.
+          destruct H3; try easy. destruct H2. destruct H2. destruct H2. inversion H2. subst. 
+          apply H3; try easy.
+          {
+            clear IHlis H3 H0 H5 H6 H7 H1 H. clear p q.
+            revert H4 H8. revert m n. clear x x0. induction lis; intros; try easy. 
+            inversion H4. inversion H8. subst. clear H4 H8.
+            specialize(IHlis m n H2 H7). constructor; try easy. clear IHlis H2 H7.
+            - destruct H1. subst. left. easy.
+            - destruct H. destruct H. destruct H. subst. right.
+              exists x. exists (incr_freeG m n x0). split; try easy.
+              apply H0.
+              destruct H6; try easy. destruct H. destruct H. destruct H. inversion H. subst. easy.
+          }
+        - destruct H. destruct H1. subst.
+          destruct H2; try easy. destruct H. destruct H. destruct H. inversion H. subst.
+          destruct H3; try easy. destruct H2. destruct H2. destruct H2. inversion H2. subst. 
+          constructor; try easy. constructor; try easy.
+          right. exists x. exists (incr_freeG m n x2).
+          split; try easy. apply H3; try easy.
+  - inversion H. subst.
+    constructor; try easy. apply IHG1; try easy.
 Qed.
   
+Lemma wfG_after_subst : forall Q G1 G2 m n,
+    wfG G1 -> wfG G2 -> subst_global m n G1 G2 Q -> wfG Q.
+Proof.
+  induction Q using global_ind_ref; intros; try easy.
+  - apply wfg_var.
+  - apply wfg_end.
+  - inversion H2; try easy. 
+    - subst.
+      apply wfG_after_incr. easy.
+    - subst. 
+      inversion H1. subst. clear H1 H2.
+      revert H H0 H8 H6 H7 H9.
+      revert p G1 m n xs q.
+      induction lis; intros; try easy. 
+      - destruct xs; try easy.
+      - destruct xs; try easy.
+        specialize(SList_f o xs H6); intros. clear H6.
+        inversion H8. subst. clear H8.
+        inversion H. subst. clear H. inversion H9. subst. clear H9.
+        destruct H1.
+        specialize(IHlis p G1 m n xs q H6 H0 H10 H H7 H8).
+        inversion IHlis; subst.
+        constructor; try easy. apply SList_b. easy.
+        constructor; try easy.
+        clear H12 H11 H8 H6 H10 H H7. 
+        destruct H4. left. easy.
+        destruct H. destruct H. destruct H. subst.
+        destruct H5; try easy. destruct H. destruct H. destruct H. destruct H. destruct H2.
+        inversion H2. subst. right. exists x1. exists x3. split; try easy. 
+        destruct H3; try easy. destruct H. destruct H. destruct H. inversion H. subst.
+        specialize(H1 G1 x0 m n). apply H1;try easy.
+      - destruct H. destruct H1. subst.
+        destruct lis; try easy. clear IHlis H10 H6 H8.
+        destruct H3; try easy. destruct H. destruct H. destruct H. inversion H. subst.
+        destruct H5; try easy. destruct H2. destruct H2. destruct H2. destruct H2. destruct H3.
+        inversion H2. subst.
+        destruct H4; try easy. destruct H3. destruct H3. destruct H3. inversion H3. subst.
+        constructor; try easy. constructor; try easy. right.
+        exists x0. exists x1. specialize(H4 G1 x2 m n). split; try easy. apply H4; try easy.
+  - inversion H1. subst.
+    apply wfG_after_incr; try easy.
+    subst.
+    specialize(IHQ G1 P (S m) (S n)). 
+    constructor. apply IHQ; try easy.
+    inversion H0. easy.
+Qed.
+  
+Lemma guard_breakG : forall x, (forall n, exists m, guardG n m (g_rec x)) -> exists T, multiS betaG (g_rec x) T /\  (forall n, exists m, guardG n m T) /\ (T = g_end \/ (exists p q lis, T = g_send p q lis)).
+Proof.
+  intros.
+  pose proof H as H1.
+  specialize(H1 1). destruct H1.
+  assert (exists T, multiS betaG (g_rec x) T /\
+  (T = g_end \/
+   (exists
+      (p q : string) (lis : seq.seq (option (sort * global))),
+      T = g_send p q lis))).
+  {
+    clear H. revert H0. revert x. induction x0; intros; try easy.
+    inversion H0. subst.
+    destruct Q; try easy.
+    - exists g_end.
+      split. apply multi_sing. constructor; try easy.
+      left. easy.
+    - exists (g_send s s0 l).
+      split. apply multi_sing. constructor; try easy.
+      right. exists s. exists s0. exists l. easy.
+    - specialize(IHx0 Q H4). 
+      destruct IHx0. destruct H. exists x1. split; try easy.
+      apply multi_step with (y := (g_rec Q)).
+      constructor; try easy.
+      easy.
+  }
+  destruct H1. destruct H1. exists x1.
+  split; try easy. split; try easy.
+  clear H0 H2. clear x0.
+  revert H. induction H1; intros; try easy.
+  - inversion H. subst.
+    specialize(H0 n). destruct H0. 
+    inversion H0. subst.
+    - exists 0. apply gg_nil.
+    - subst. exists m.
+      specialize(subst_injG 0 0 (g_rec G) G y Q H3 H1); intros. subst. easy.
+  - inversion H. subst.
+    apply IHmultiS; try easy.
+    intros. specialize(H0 n0). destruct H0.
+    inversion H0. subst. exists 0. apply gg_nil.
+    subst. exists m.
+    specialize(subst_injG 0 0 (g_rec G) G y Q H4 H2); intros. subst. easy.
+Qed.
+
 
 End gtt.
+
 
 
 
