type/examples.v
@@ -1,0 +1,24 @@
+From SST Require Export src.expressions process.processes process.typecheck type.global type.local process.beta process.sessions process.inversion  type.isomorphism type.projection type.proj_sub.
+Require Import String List Datatypes ZArith Relations PeanoNat.
+From Paco Require Import paco pacotac.
+Require Import Setoid Morphisms Coq.Program.Basics.
+Require Import Coq.Init.Datatypes.
+Open Scope list_scope.
+Import ListNotations.
+
+CoFixpoint Ga : gtt := gtt_send "Alice" "Bob" [Some (snat, Ga)].
+
+Example Grec : gttTC (g_rec (g_send "Alice" "Bob" [Some (snat, g_var 0)])) Ga.
+Proof.
+  pcofix CIH.
+  pfold. apply gttT_rec with (Q := g_send "Alice" "Bob" [(Some (snat, (g_rec (g_send "Alice" "Bob" [Some (snat, g_var 0)]))))]).
+  constructor. constructor. right.
+  exists snat. exists (g_var 0). exists (g_rec (g_send "Alice" "Bob" [Some (snat, g_var 0)])).
+  split; try easy. split; try easy. constructor. easy.
+  
+  rewrite (gtt_eq Ga). simpl.
+  left. pfold.
+  constructor. constructor. right. exists snat. exists (g_rec (g_send "Alice" "Bob" [Some (snat, g_var 0)])). exists Ga.
+  split; try easy. split; try easy.
+  right. easy. easy.
+Qed.
